cfrontend/Initializers.v
@@ -110,7 +110,7 @@ Fixpoint constval (ce: composite_env) (a: expr) : res val :=
   | Ecomma r1 r2 ty =>
       do v1 <- constval ce r1; constval ce r2
   | Evar x ty =>
-      OK(Vptr x Ptrofs.zero)
+      OK(Vptr (Block.glob x) Ptrofs.zero)
   | Ederef r ty =>
       constval ce r
   | Efield l f ty =>
@@ -163,9 +163,20 @@ Definition transl_init_single (ce: composite_env) (ty: type) (a: expr) : res ini
   | Vlong n, Tpointer _ _ => assertion (Archi.ptr64); OK(Init_int64 n)
   | Vsingle f, Tfloat F32 _ => OK(Init_float32 f)
   | Vfloat f, Tfloat F64 _ => OK(Init_float64 f)
-  | Vptr id ofs, Tint I32 sg _ => assertion (negb Archi.ptr64); OK(Init_addrof id ofs)
-  | Vptr id ofs, Tlong _ _ => assertion (Archi.ptr64); OK(Init_addrof id ofs)
-  | Vptr id ofs, Tpointer _ _ => OK(Init_addrof id ofs)
+  | Vptr id ofs, Tint I32 sg _ => assertion (negb Archi.ptr64);
+                                   match Block.ident_of id with
+                                     Some i => OK(Init_addrof i ofs)
+                                   | _ => Error (msg "Vptr should be a global in initializer")
+                                   end
+  | Vptr id ofs, Tlong _ _ => assertion (Archi.ptr64);
+                               match Block.ident_of id with
+                                 Some i => OK(Init_addrof i ofs)
+                               | _ => Error (msg "Vptr should be a global in initializer")
+                               end
+  | Vptr id ofs, Tpointer _ _ => match Block.ident_of id with
+                                  Some i => OK(Init_addrof i ofs)
+                                | _ => Error (msg "Vptr should be a global in initializer")
+                                end
   | Vundef, _ => Error(msg "undefined operation in initializer")
   | _, _ => Error (msg "type mismatch in initializer")
   end.
